WIP

code/ecdsap256/Hacl.Impl.P256.Q.CR.fst
@@ -9,29 +9,31 @@ open Lib.IntTypes
 open Lib.Buffer
 
 
+#set-options "--z3rlimit 300" 
+
+
 open Hacl.Impl.P256.LowLevel
 
 let pointLen = 8ul
 
 (*cmovznz *)
 val select: r: lbuffer uint64 pointLen 
-  -> points: lbuffer uint64 (pointLen *. 16ul) 
-  -> id0: size_t
-  -> id1: size_t 
+  -> a: lbuffer uint64 pointLen
+  -> b: lbuffer uint64 pointLen
   -> bit: uint8 {v bit = 0 \/ v bit = 1} 
   -> Stack unit 
-    (requires fun h -> True)
+    (requires fun h ->  live h r /\ live h a /\ live h b)
     (ensures fun h0 _ h1 -> modifies (loc r) h0 h1)
 
-let select r points id0 id1 bit = 
+let select r a b bit = 
   let x = sub r (size 0) (size 4) in 
   let y = sub r (size 4) (size 4) in 
 
-  let pX = sub points (id0 *. pointLen) (size 4) in 
-  let pY = sub points ((id0 +. 1ul) *. pointLen) (size 4) in 
+  let pX = sub a (size 0) (size 4) in 
+  let pY = sub a (size 4) (size 4) in  
 
-  let qX = sub points (id1 *. pointLen) (size 4) in 
-  let qY = sub points ((id1 +. 1ul) *. pointLen) (size 4) in 
+  let qX = sub b (size 0) (size 4) in 
+  let qY = sub b (size 4) (size 4) in  
 
   let bitAsUInt64 = to_u64 bit in 
 
@@ -40,21 +42,71 @@ let select r points id0 id1 bit =
 
 
 
-val do_lookup: a: lbuffer uint64 (pointLen *. 16ul) -> scalar: uint8 {v scalar < 16} -> Stack unit
-  (requires fun h -> True)
+val do_lookup: result: lbuffer uint64 pointLen ->  a: lbuffer uint64 (pointLen *. 16ul) -> scalar: uint8 {v scalar < 16} -> 
+Stack unit
+  (requires fun h -> live h result /\ live h a)
   (ensures fun h0 _ h1 -> True)
 
-let do_lookup a scalar =
+let do_lookup result a scalar =
   push_frame();
     let tn = create (pointLen *. 14ul) (u64 0) in 
 
     let t0_0 = sub tn (size 0) pointLen in 
-  
-    let b0 = logand scalar (1uy) in 
-    let id0_0 = 0ul in 
-    let id1_0 = 1ul in 
+    let t0_1 = sub tn pointLen pointLen in 
+    let t0_2 = sub tn (2ul *. pointLen) pointLen in 
+    let t0_3 = sub tn (3ul *. pointLen) pointLen in 
+    let t0_4 = sub tn (4ul *. pointLen) pointLen in 
+    let t0_5 = sub tn (5ul *. pointLen) pointLen in 
+    let t0_6 = sub tn (6ul *. pointLen) pointLen in 
+    let t0_7 = sub tn (7ul *. pointLen) pointLen in 
 
-  (* for i in range(0...n) *)
-    select t0_0 a id0_0 id1_0 b0;
+    let t1_0 = sub tn (8ul *. pointLen) pointLen in 
+    let t1_1 = sub tn (9ul *. pointLen) pointLen in 
+    let t1_2 = sub tn (10ul *. pointLen) pointLen in 
+    let t1_3 = sub tn (11ul *. pointLen) pointLen in 
+
+    let t2_0 = sub tn (12ul *. pointLen) pointLen in 
+    let t2_1 = sub tn (13ul *. pointLen) pointLen in 
+  
+    let b0 = logand scalar 1uy in 
+    let b1 = logand scalar 2uy in 
+    let b2 = logand scalar 4uy in 
+    let b3 = logand scalar 8uy in 
+
+    select t0_0 (sub a (size 0) pointLen) (sub a (size 1 *. pointLen) pointLen) b0;
+    select t0_1 (sub a (size 2 *. pointLen) pointLen) (sub a (size 3 *. pointLen) pointLen) b0;
+    select t0_2 (sub a (size 4 *. pointLen) pointLen) (sub a (size 5 *. pointLen) pointLen) b0;
+    select t0_3 (sub a (size 6 *. pointLen) pointLen) (sub a (size 7 *. pointLen) pointLen) b0;
+    select t0_4 (sub a (size 8 *. pointLen) pointLen) (sub a (size 9 *. pointLen) pointLen) b0;
+    select t0_5 (sub a (size 10 *. pointLen) pointLen) (sub a (size 11 *. pointLen) pointLen) b0;
+    select t0_6 (sub a (size 12 *. pointLen) pointLen) (sub a (size 13 *. pointLen) pointLen) b0;
+    select t0_7 (sub a (size 14 *. pointLen) pointLen) (sub a (size 15 *. pointLen) pointLen) b0;
+
+    select t1_0 t0_0 t0_1 b1;
+    select t1_1 t0_2 t0_3 b1;
+    select t1_2 t0_4 t0_5 b1;
+    select t1_3 t0_6 t0_6 b1;
+
+    select t2_0 t1_0 t1_1 b2;
+    select t2_1 t1_2 t1_3 b2;
+
+    select result t2_0 t2_1 b3;
     
   pop_frame()
+
+open Spec.P256.Definitions
+
+inline_for_extraction noextract 
+val ml_r2_step: #buf_type: buftype -> 
+  p: point -> q: point ->tempBuffer: lbuffer uint64 (size 88) -> 
+  scalar: lbuffer_t buf_type uint8 (size 32) -> 
+  i:size_t{v i < 256} -> 
+  Stack unit
+  (requires fun h -> live h p /\ live h q /\ live h tempBuffer /\ live h scalar /\
+    LowStar.Monotonic.Buffer.all_disjoint [loc p; loc q; loc tempBuffer; loc scalar])
+  (ensures fun h0 _ h1 -> True)
+
+(*
+let ml_r2_step #buf_type p q tempBuffer scalar i = 
+  let bit0 = (size 255) -. i in 
+  
